paxos/proof.dfy
@@ -1,0 +1,50 @@
+include "types.dfy"
+include "network.dfy"
+include "agents.dfy"
+include "synod.dfy"
+
+module Proof {
+import opened Network
+import opened Agents
+import opened Types
+import opened Synod
+
+
+/* If all processes propose v, then every process that decides a value decides v */
+predicate Validity(ds:DistrSys) {
+    (exists v :: AllProcessesProposeV(ds, v)) 
+    ==> 
+    (exists v :: AllProcessesProposeV(ds, v) && AllDecidedProcessesDecidesV(ds, v)) 
+}
+
+predicate AllProcessesProposeV(ds:DistrSys, v:Value) {
+    forall l | l in ds.leaders :: l.consts.initval == v
+}
+
+predicate AllDecidedProcessesDecidesV(ds:DistrSys, v:Value){
+    forall l | l in ds.leaders && l.state == Decided :: l.val == v
+}
+
+
+predicate Validity_Inv(ds:DistrSys) {
+    && Validity(ds)
+}
+
+
+lemma InitImpliesInv(ds:DistrSys, f:nat, l:nat, accConf:seq<Id>) 
+    requires Init(ds, f, l, accConf)
+    ensures Validity_Inv(ds)
+{}
+
+lemma NextPreservesInv(ds:DistrSys, ds':DistrSys) 
+    requires Validity_Inv(ds)
+    requires Next(ds, ds')
+    ensures Validity_Inv(ds')
+{
+    // TODO
+    assume false;
+}
+
+
+
+}
